tests/TestsSV.hs
@@ -18,8 +18,11 @@ module Main where
 
 import Cava2SystemVerilog
 import Instantiate
+import TestMultiply
 
 main :: IO ()
 main = do writeSystemVerilog instantiateNetlist
           writeTestBench instantiate_tb
+          writeSystemVerilog mult2_3_5Netlist
+          writeTestBench mult2_3_5_tb
 
