tests/TestMultiply.v
@@ -1,0 +1,81 @@
+(****************************************************************************)
+(* Copyright 2020 The Project Oak Authors                                   *)
+(*                                                                          *)
+(* Licensed under the Apache License, Version 2.0 (the "License")           *)
+(* you may not use this file except in compliance with the License.         *)
+(* You may obtain a copy of the License at                                  *)
+(*                                                                          *)
+(*     http://www.apache.org/licenses/LICENSE-2.0                           *)
+(*                                                                          *)
+(* Unless required by applicable law or agreed to in writing, software      *)
+(* distributed under the License is distributed on an "AS IS" BASIS,        *)
+(* WITHOUT WARRANTIES OR CONDITIONS OF ANY KIND, either express or implied. *)
+(* See the License for the specific language governing permissions and      *)
+(* limitations under the License.                                           *)
+(****************************************************************************)
+
+From Coq Require Import Ascii String.
+From Coq Require Import Bool.Bool.
+From Coq Require Import NArith.
+From Coq Require Import Lists.List.
+Import ListNotations.
+
+Require Import ExtLib.Structures.Monads.
+Export MonadNotation.
+
+From Coq Require Vector.
+From Coq Require Import Bool.Bvector.
+
+Require Import Omega.
+
+Require Import Cava.Cava.
+Require Import Cava.Monad.CavaMonad.
+
+Definition bv2_0  := N2Bv_sized 2  0.
+Definition bv2_3  := N2Bv_sized 2  3.
+Definition bv3_0  := N2Bv_sized 3  0.
+Definition bv3_5  := N2Bv_sized 3  5.
+Definition bv3_7  := N2Bv_sized 3  7.
+Definition bv5_15 := N2Bv_sized 5 15.
+
+(* Check 3 * 5 = 30 *)
+Example mult3_5 : combinational (unsignedMult bv2_3 bv3_5) = bv5_15.
+Proof. reflexivity. Qed.
+
+(* A top-level multiplier circuit that can be compiled to a top-level
+   SystemVerilog circuit. *)
+Definition multiplier {m bit} `{Cava m bit} {aSize bSize: nat}
+                      (ab: Vector.t bit aSize * Vector.t bit bSize) :
+                      m (Vector.t bit (aSize + bSize)) :=
+  let (a, b) := ab in
+  unsignedMult a b.
+
+(* Check 3 * 5 = 30 *)
+Example mult3_5_top : combinational (multiplier (bv2_3, bv3_5)) = bv5_15.
+Proof. reflexivity. Qed.
+
+(******************************************************************************)
+(* Generate an unsigned multiplier with 2 and 3 bit inputs and 5-bit result.  *)
+(******************************************************************************)
+
+Local Open Scope nat_scope.
+
+Definition mult2_3_5Interface
+  := combinationalInterface "mult2_3_5"
+     (mkPort "a" (Vec Bit 2), mkPort "b" (Vec Bit 3))
+     (mkPort "product" (Vec Bit 5))
+     [].
+
+Definition mult2_3_5Netlist
+  := makeNetlist mult2_3_5Interface multiplier.
+
+Definition mult2_3_5_tb_inputs
+  := [(bv2_3, bv3_5); (bv2_3, bv3_7); (bv2_0, bv3_0)].
+
+Definition mult2_3_5_tb_expected_outputs
+  := map (fun ab => combinational (multiplier ab)) mult2_3_5_tb_inputs.
+
+Definition  mult2_3_5_tb
+  := testBench "mult2_3_5_tb" mult2_3_5Interface
+     mult2_3_5_tb_inputs mult2_3_5_tb_expected_outputs.
+
